Test/BadGenExec.lean
@@ -1,4 +1,9 @@
 import Veil
+import Veil.Core.Tools.ModelChecker.TransitionSystem
+import Veil.Core.Tools.ModelChecker.Interface
+import Veil.Core.Tools.ModelChecker.Concrete.Checker
+import Mathlib.Data.FinEnum
+import Mathlib.Tactic.ProxyType
 
 -- https://github.com/aman-goel/ivybench/blob/5db7eccb5c3bc2dd14dfb58eddb859b036d699f5/ex/ivy/ring.ivy
 
@@ -7,56 +12,59 @@ set_option trace.veil.desugar true
 veil module Ring
 
 type node
-type foo
+-- type foo
 
-inductive Action (node : Type) where
-  | send (n next : node)
-  | recv (sender n next : node)
-deriving Inhabited, Ord, Lean.ToJson, Hashable, BEq
+-- inductive Action (node : Type) where
+--   | send (n next : node)
+--   | recv (sender n next : node)
+-- deriving Inhabited, Ord, Lean.ToJson, Hashable, BEq, Repr
 
 instantiate tot : TotalOrder node
 instantiate btwn : Between node
+-- -- set_option synthInstance.maxHeartbeats 200000ʡ
+-- -- FIXME: importing `ModelChecker.TransitionSystem` causes this to break???
+-- -- It was because of `class abbrev Collection`
+-- enum Guest = {Olivier, Bruno, Aquinas}
 
-enum Guest = {Olivier, Bruno, Aquinas}
+-- instance : Std.LawfulEqCmp (Ord.compare (self := inferInstanceAs (Ord Guest_IndT))) :=
+--  by apply Std.LawfulEqCmp.mk; decide
 
 open Between TotalOrder
 
 
-immutable individual foobar : foo
+-- immutable individual foobar : foo
 
-individual log : List (Action node)
+-- individual log : List (Action node)
 relation leader : node -> Bool
 relation pending : node -> node -> Bool
-relation pendingfff : node → foo → Bool
+-- relation pendingfff : node → foo → Bool
 -- NOTE: this causes the issue with deriving the FieldRepresentation and
 -- LawfulFieldRepresentation instances commenting it out makes this file compile
 -- successfully
-function zz : node → foo → node → node
+-- function zz : node → foo → node → node
 #time #gen_state
 
 after_init {
-  log := []
+  -- log := []
   leader N := false
   pending M N := false
 }
 
-#check Veil.Enumeration
-
 action send (n next : node) {
   require ∀ Z, n ≠ next ∧ ((Z ≠ n ∧ Z ≠ next) → btw n next Z)
-  log := log ++ [Action.send n next]
+  -- log := log ++ [Action.send n next]
   pending n next := true
 }
 
 action recv (sender n next : node) {
   require ∀ Z, n ≠ next ∧ ((Z ≠ n ∧ Z ≠ next) → btw n next Z)
   require pending sender n
-  log := log ++ [Action.recv sender n next]
+  -- log := log ++ [Action.recv sender n next]
   -- message may or may not be removed
   -- this models that multiple messages might be in flight
   let b ← pick Bool
   pending sender n := b  -- FIXME: `pending sender n := *` has bad execution performance
-  if (n = n) then
+  if (sender = n) then
     leader n := true
   else
     -- pass message to next node
@@ -78,14 +86,123 @@ invariant pending L L → le N L
 
 #check_invariants
 
-#time #finitize_types (Fin 5), (Fin 3), Guest_IndT
-#set_theory { foobar := 0 }
 
-#time #model_check single_leader
-#eval spaceSize modelCheckerResult
+#check Theory
+#check State
+#check FieldConcreteType
+#check Label
 
-open ProofWidgets
-open scoped ProofWidgets.Jsx
-#html <ModelCheckerView trace={statesJson} layout={"vertical"} />
+abbrev node := Fin 5
+-- abbrev foo := Fin 1
+-- abbrev Guest := Guest_IndT
+
+#check Veil.EnumerableTransitionSystem
+
+-- simple_deriving_repr_for Theory
+simple_deriving_repr_for' State
+
+
+abbrev CTheory := Theory node -- foo Guest
+abbrev CFieldType := FieldConcreteType node -- foo Guest
+abbrev CState := State CFieldType
+abbrev CLabel := Label node -- foo Guest
+
+-- instance : Repr CTheory := inferInstance
+instance : Repr CLabel := inferInstance
+
+instance : Repr CState := inferInstance
+
+
+deriving instance DecidableEq for Label
+deriving instance BEq, Repr for Theory
+
+instance : Veil.Enumeration CLabel where
+  allValues := (FinEnum.ofEquiv _ (Equiv.symm (proxy_equiv% CLabel))).toList
+  complete := by simp
+
+abbrev CInit := initMultiExec CTheory CState node CFieldType -- foo Guest CFieldType
+abbrev CNext := nextActMultiExec CTheory CState node -- foo Guest
+
+/-- Extract the resulting state from an ExceptT-wrapped execution, if successful. -/
+def getStateFromExceptT (c : ExceptT ε DivM (α × σ)) : Option σ :=
+  match c.run with
+  | .res (.ok (_, st)) => .some st
+  | .res (.error _)    => .none
+  | .div => none
+
+def getAllStatesFromExceptT (c : List (ExceptT ε DivM (α × σ))) : List (Option σ) :=
+  c.map getStateFromExceptT
+
+/-- Extract all valid states from a VeilMultiExecM computation -/
+def extractValidStates (exec : Veil.VeilMultiExecM κᵣ ℤ ρ σ Unit) (rd : ρ) (st : σ) : List (Option σ) :=
+  exec rd st |>.map Prod.snd |> getAllStatesFromExceptT
+
+def xx : Veil.Enumeration CLabel := inferInstance
+#eval xx.allValues
+
+@[specialize]
+def enumerableTransitionSystem [labels : Veil.Enumeration CLabel] :
+  Veil.EnumerableTransitionSystem
+  CTheory (List CTheory)
+  CState (List CState)
+  CLabel
+  (List (CLabel × CState)) where
+  theories := [{} /-{foobar := 0}-/]
+  initStates := fun th =>
+    extractValidStates CInit th default |>.filterMap id
+  tr := fun th st =>
+    labels.allValues.flatMap (fun l =>
+      (extractValidStates (CNext l) th st |>.filterMap id).map (fun next => (l, next)))
+
+abbrev Th : CTheory := {/-foobar := 0-/ }
+abbrev HTh : Th ∈ enumerableTransitionSystem.theories := by apply List.Mem.head
+
+open Veil.ModelChecker
+abbrev SearchParams : SearchParameters CTheory CState := {
+  «safety» := {
+    name := `single_leader
+    property := fun th st => single_leader th st
+    decidable := inferInstance
+  }
+  earlyTerminationConditions := [
+    EarlyTerminationCondition.foundViolatingState
+  ]
+}
+
+abbrev Hash := UInt64
+
+-- deriving instance LawfulBEq for UInt64
+
+-- instance : LawfulBEq UInt64 := inferInstance
+-- instance : LawfulHashable UInt64 := inferInstance
+
+-- set_option synthInstance.maxHeartbeats 1000000
+-- set_option trace.Meta.synthInstance true
+-- instance : Concrete.StateFingerprint CState UInt64 := inferInstance
+
+#check Concrete.findReachable
+
+
+def modelCheckerResult :=
+
+  @Concrete.findReachable CTheory CState CLabel Hash
+  (Concrete.StateFingerprint.ofHash CState)
+  _ _ _ _ _ _ _
+  enumerableTransitionSystem Th HTh SearchParams
+
+#time #eval! modelCheckerResult
+
+
+  -- Concrete.findReachable enumerableTransitionSystem Th HTh SearchParams
+
+-- #time #finitize_types (Fin 5), (Fin 3), Guest_IndT
+-- #set_theory { foobar := 0 }
+
+-- #time #model_check single_leader
+-- #eval spaceSize modelCheckerResult
+
+-- open ProofWidgets
+-- open scoped ProofWidgets.Jsx
+-- #html <ModelCheckerView trace={statesJson} layout={"vertical"} />
 
 end Ring
