Veil/Core/Tools/ModelChecker/Concrete/Checker.lean
@@ -10,17 +10,20 @@ open Std
 class StateView (FullState View : Type) where
   view : FullState → View
 
-@[default_instance low] instance : StateView σ σ where
-  view := id
-
 class abbrev StateFingerprint (FullState View : Type) := BEq View, LawfulBEq View, Hashable View, LawfulHashable View, StateView FullState View
+
+def StateFingerprint.ofHash (σ : Type) [Hashable σ] : StateFingerprint σ UInt64 where
+  beq := BEq.beq
+  rfl := BEq.rfl
+  eq_of_beq := LawfulBEq.eq_of_beq
+  hash_eq := LawfulHashable.hash_eq
+  view := hash
 
 /-- A model checker search context is parametrised by the system that's being
 checked and the theory it's being checked under. -/
-structure SearchContext {ρ σ κ σₕ : Type} (SetT : Type → Type)
-  [Collection SetT ρ] [Collection SetT σ] [Collection SetT (κ × σ)]
+structure SearchContext {ρ σ κ σₕ : Type}
   [fp : StateFingerprint σ σₕ]
-  (sys : EnumerableTransitionSystem ρ (SetT ρ) σ (SetT σ) κ (SetT (κ × σ)))
+  (sys : EnumerableTransitionSystem ρ (List ρ) σ (List σ) κ (List (κ × σ)))
   (th : ρ) (hTh : th ∈ sys.theories)
   (params : SearchParameters ρ σ)
 where
@@ -31,20 +34,19 @@ where
   log                : Std.HashMap σₕ (σₕ × κ)
   violatingStates    : List σₕ
   /-- Have we finished the search? If so, why? -/
-  finished           : Option StoppingCondition
+  finished           : Option TerminationReason
   queue_sound        : ∀ x : σ, ⟨fp.view x, x⟩ ∈ fQueue.toList sq → sys.reachable th x
   visited_sound      : Function.Injective fp.view → ∀ x, (fp.view x) ∈ seen → sys.reachable th x
   queue_sub_visited  : ∀ x : σ, ⟨fp.view x, x⟩ ∈ fQueue.toList sq → (fp.view x) ∈ seen
   queue_wellformed   : ∀ fingerprint st, ⟨fingerprint, st⟩ ∈ fQueue.toList sq → fingerprint = fp.view st
 
 @[inline, specialize]
-def SearchContext.hasFinished {ρ σ κ σₕ : Type} {SetT : Type → Type}
-  [Collection SetT ρ] [Collection SetT σ] [Collection SetT (κ × σ)]
+def SearchContext.hasFinished {ρ σ κ σₕ : Type}
   [fp : StateFingerprint σ σₕ]
-  [sys : EnumerableTransitionSystem ρ (SetT ρ) σ (SetT σ) κ (SetT (κ × σ))]
+  (sys : EnumerableTransitionSystem ρ (List ρ) σ (List σ) κ (List (κ × σ)))
   {th : ρ} {hTh : th ∈ sys.theories}
   (params : SearchParameters ρ σ)
-  (ctx : @SearchContext ρ σ κ σₕ SetT _ _ _ fp sys th hTh params) : Bool := ctx.finished.isSome
+  (ctx : @SearchContext ρ σ κ σₕ fp sys th hTh params) : Bool := ctx.finished.isSome
 
 def SearchContext.initial {ρ σ κ σₕ : Type}
   [fp : StateFingerprint σ σₕ]
@@ -52,7 +54,7 @@ def SearchContext.initial {ρ σ κ σₕ : Type}
   (sys : EnumerableTransitionSystem ρ (List ρ) σ (List σ) κ (List (κ × σ)))
   (th : ρ) (hTh : th ∈ sys.theories)
   (params : SearchParameters ρ σ) :
-  @SearchContext ρ σ κ σₕ List _ _ _ fp sys th hTh params := {
+  @SearchContext ρ σ κ σₕ fp sys th hTh params := {
     seen := HashSet.insertMany HashSet.emptyWithCapacity (sys.initStates th |> Functor.map fp.view),
     sq := fQueue.ofList (sys.initStates th |> Functor.map (fun s => (fp.view s, s))),
     log := Std.HashMap.emptyWithCapacity
@@ -62,8 +64,8 @@ def SearchContext.initial {ρ σ κ σₕ : Type}
     visited_sound := by
       dsimp only [Functor.map]
       intro h_view_inj x h_in
-      have h_in_init : x ∈ (EnumerableTransitionSystem.initStates σ (List (κ × σ)) th) := by {
-        have h_in_list : fp.view x ∈ ((EnumerableTransitionSystem.initStates σ (List (κ × σ)) th)).map fp.view := by
+      have h_in_init : x ∈ sys.initStates th := by {
+        have h_in_list : fp.view x ∈ (sys.initStates th).map fp.view := by
           { grind [Std.HashSet.mem_of_mem_insertMany_list] }
         rw [List.mem_map] at h_in_list
         obtain ⟨s, h_s_in, h_eq_view⟩ := h_in_list
@@ -76,21 +78,18 @@ def SearchContext.initial {ρ σ κ σₕ : Type}
   }
 
 @[inline, specialize]
-def SearchContext.shouldStop {ρ σ κ σₕ : Type} {SetT : Type → Type}
-  [Collection SetT ρ] [Collection SetT σ] [Collection SetT (κ × σ)]
+def SearchContext.shouldTerminateEarly {ρ σ κ σₕ : Type}
   [fp : StateFingerprint σ σₕ]
-  [sys : EnumerableTransitionSystem ρ (SetT ρ) σ (SetT σ) κ (SetT (κ × σ))]
+  (sys : EnumerableTransitionSystem ρ (List ρ) σ (List σ) κ (List (κ × σ)))
   {th : ρ} {hTh : th ∈ sys.theories}
   {params : SearchParameters ρ σ}
-  (ctx : @SearchContext ρ σ κ σₕ SetT _ _ _ fp sys th hTh params)
+  (ctx : @SearchContext ρ σ κ σₕ fp sys th hTh params)
   (currSt : σ)
-  : Option StoppingCondition :=
-  ctx.finished.orElse (fun () =>
-    params.stoppingConditions.findSome? (fun sc => match sc with
-    | StoppingCondition.exploredAllReachableStates => if ctx.sq.dequeue?.isNone then some sc else none
-    | StoppingCondition.foundViolatingState => if !params.safety.holdsOn th currSt then some sc else none
-  ))
-
+  : Option EarlyTerminationCondition :=
+  match ctx.finished with
+  | some (.earlyTermination condition) => some condition
+  | _ => params.earlyTerminationConditions.findSome? (fun sc => match sc with
+    | EarlyTerminationCondition.foundViolatingState => if !params.safety.holdsOn th currSt then some sc else none)
 
 /-- Process a single neighbor node during BFS traversal.
 If the neighbor has been seen, return the current context unchanged.
@@ -99,19 +98,19 @@ Otherwise, add it to seen set and log, then enqueue it. -/
 def SearchContext.tryExploreNeighbor {ρ σ κ σₕ : Type}
   [fp : StateFingerprint σ σₕ]
   [BEq ρ] [BEq σ] [BEq κ]
-  [sys : EnumerableTransitionSystem ρ (List ρ) σ (List σ) κ (List (κ × σ))]
+  (sys : EnumerableTransitionSystem ρ (List ρ) σ (List σ) κ (List (κ × σ)))
   {th : ρ} {hTh : th ∈ sys.theories}
   {params : SearchParameters ρ σ}
   (fpSt : σₕ)  -- fingerprint of state we're coming from (pre-state), for logging
-  (ctx : @SearchContext ρ σ κ σₕ List _ _ _ fp sys th hTh params)
+  (ctx : @SearchContext ρ σ κ σₕ fp sys th hTh params)
   (neighbor : κ × σ)
   (h_neighbor : sys.reachable th neighbor.2) :
-  @SearchContext ρ σ κ σₕ List _ _ _ fp sys th hTh params :=
+  @SearchContext ρ σ κ σₕ fp sys th hTh params :=
   let ⟨label, succ⟩ := neighbor
   let fingerprint := fp.view succ
   if ctx.seen.contains fingerprint then ctx
   else
-    let ctx_with_seen : @SearchContext ρ σ κ σₕ List _ _ _ fp sys th hTh params := {
+    let ctx_with_seen : @SearchContext ρ σ κ σₕ fp sys th hTh params := {
       ctx with
         seen := ctx.seen.insert fingerprint,
         log := ctx.log.insert fingerprint (fpSt, label),
@@ -131,43 +130,43 @@ def SearchContext.tryExploreNeighbor {ρ σ κ σₕ : Type}
 @[inline, specialize]
 def SearchContext.processState {ρ σ κ σₕ : Type}
   [fp : StateFingerprint σ σₕ]
-  [BEq ρ] [BEq σ] [BEq κ]
-  [sys : EnumerableTransitionSystem ρ (List ρ) σ (List σ) κ (List (κ × σ))]
+  [BEq ρ] [BEq σ] [BEq κ] [Repr σ] [Repr σₕ]
+  (sys : EnumerableTransitionSystem ρ (List ρ) σ (List σ) κ (List (κ × σ)))
   {th : ρ} {hTh : th ∈ sys.theories}
   {params : SearchParameters ρ σ}
   (fpSt : σₕ)
   (curr : σ)
   (h_curr : sys.reachable th curr)
-  (ctx : @SearchContext ρ σ κ σₕ List _ _ _ fp sys th hTh params) :
-  @SearchContext ρ σ κ σₕ List _ _ _ fp sys th hTh params :=
-  -- Check whether we should stop the search
-  match ctx.shouldStop curr with
-  | some .foundViolatingState => {ctx with finished := some .foundViolatingState, violatingStates := fpSt :: ctx.violatingStates}
-  | some .exploredAllReachableStates => {ctx with finished := some .exploredAllReachableStates}
+  (ctx : @SearchContext ρ σ κ σₕ fp sys th hTh params) :
+  @SearchContext ρ σ κ σₕ fp sys th hTh params :=
+  -- Check whether we should stop the search early
+  match ctx.shouldTerminateEarly sys curr with
+  | some .foundViolatingState => {ctx with finished := some (.earlyTermination .foundViolatingState), violatingStates := fpSt :: ctx.violatingStates}
   -- If not, explore all neighbors of the current state
-  | none => (sys.tr th curr).attach.foldl (fun current_ctx ⟨⟨tr, postState⟩, h_neighbor_in_tr⟩ =>
+  | none =>
+    (sys.tr th curr).attach.foldl (fun current_ctx ⟨⟨tr, postState⟩, h_neighbor_in_tr⟩ =>
     if current_ctx.hasFinished then current_ctx
     else
       let h_neighbor_reachable : sys.reachable th postState :=
         EnumerableTransitionSystem.reachable.step curr postState h_curr ⟨tr, h_neighbor_in_tr⟩
-      SearchContext.tryExploreNeighbor fpSt current_ctx ⟨tr, postState⟩ h_neighbor_reachable
+      SearchContext.tryExploreNeighbor sys fpSt current_ctx ⟨tr, postState⟩ h_neighbor_reachable
   ) ctx
 
 /-- Perform one step of BFS. -/
 @[inline, specialize]
 def SearchContext.bfsStep {ρ σ κ σₕ : Type}
   [fp : StateFingerprint σ σₕ]
-  [BEq ρ] [BEq σ] [BEq κ]
-  [sys : EnumerableTransitionSystem ρ (List ρ) σ (List σ) κ (List (κ × σ))]
+  [BEq ρ] [BEq σ] [BEq κ] [Repr σ] [Repr σₕ]
+  (sys : EnumerableTransitionSystem ρ (List ρ) σ (List σ) κ (List (κ × σ)))
   {th : ρ} {hTh : th ∈ sys.theories}
   {params : SearchParameters ρ σ}
-  (ctx : @SearchContext ρ σ κ σₕ List _ _ _ fp sys th hTh params) :
-  @SearchContext ρ σ κ σₕ List _ _ _ fp sys th hTh params :=
+  (ctx : @SearchContext ρ σ κ σₕ fp sys th hTh params) :
+  @SearchContext ρ σ κ σₕ fp sys th hTh params :=
   match ctx.sq.dequeue? with
-  | none => { ctx with finished := StoppingCondition.exploredAllReachableStates }
+  | none => { ctx with finished := some (.exploredAllReachableStates) }
   | some ((fpSt, curr), q_tail) =>
     have h_curr : sys.reachable th curr := sorry
-    let ctx_dequeued : @SearchContext ρ σ κ σₕ List _ _ _ fp sys th hTh params := {
+    let ctx_dequeued : @SearchContext ρ σ κ σₕ fp sys th hTh params := {
       ctx with
         sq := q_tail,
         queue_sound := sorry
@@ -175,19 +174,19 @@ def SearchContext.bfsStep {ρ σ κ σₕ : Type}
         queue_sub_visited := sorry
         queue_wellformed := sorry
     }
-    SearchContext.processState fpSt curr h_curr ctx_dequeued
+    SearchContext.processState sys fpSt curr h_curr ctx_dequeued
 
 @[specialize]
 def breadthFirstSearch {ρ σ κ σₕ : Type}
   [fp : StateFingerprint σ σₕ]
-  [BEq ρ] [BEq σ] [BEq κ]
-  [sys : EnumerableTransitionSystem ρ (List ρ) σ (List σ) κ (List (κ × σ))]
+  [BEq ρ] [BEq σ] [BEq κ] [Repr σ] [Repr σₕ]
+  (sys : EnumerableTransitionSystem ρ (List ρ) σ (List σ) κ (List (κ × σ)))
   (th : ρ) (hTh : th ∈ sys.theories)
   (params : SearchParameters ρ σ) :
-  @SearchContext ρ σ κ σₕ List _ _ _ fp sys th hTh params := Id.run do
-  let mut ctx : @SearchContext ρ σ κ σₕ List _ _ _ fp sys th hTh params := SearchContext.initial sys th hTh params
+  @SearchContext ρ σ κ σₕ fp sys th hTh params := Id.run do
+  let mut ctx : @SearchContext ρ σ κ σₕ fp sys th hTh params := SearchContext.initial sys th hTh params
   while !ctx.hasFinished do
-    ctx := SearchContext.bfsStep ctx
+    ctx := SearchContext.bfsStep sys ctx
   return ctx
 
 /-! ## Trace Recovery
@@ -213,13 +212,12 @@ def findByFingerprint [fp : StateFingerprint σ σₕ]
   states.find? (fun s => fp.view s == targetFp) |>.getD fallback
 
 /-- Extract fingerprint traces for all violating states in a SearchContext. -/
-def collectTraces {ρ σ κ σₕ : Type} {SetT : Type → Type}
-  [Collection SetT ρ] [Collection SetT σ] [Collection SetT (κ × σ)]
+def collectTraces {ρ σ κ σₕ : Type}
   [fp : StateFingerprint σ σₕ]
-  {sys : EnumerableTransitionSystem ρ (SetT ρ) σ (SetT σ) κ (SetT (κ × σ))}
+  {sys : EnumerableTransitionSystem ρ (List ρ) σ (List σ) κ (List (κ × σ))}
   {th : ρ} {hTh : th ∈ sys.theories}
   {params : SearchParameters ρ σ}
-  (ctx : @SearchContext ρ σ κ σₕ SetT _ _ _ fp sys th hTh params)
+  (ctx : @SearchContext ρ σ κ σₕ fp sys th hTh params)
   : List (σₕ × List (Step σₕ κ)) :=
   ctx.violatingStates.map (fun badState => retraceSteps ctx.log badState)
 
@@ -232,7 +230,7 @@ def recoverTrace {ρ σ κ σₕ : Type}
   (sys : EnumerableTransitionSystem ρ (List ρ) σ (List σ) κ (List (κ × σ)))
   (th : ρ) (hTh : th ∈ sys.theories)
   (params : SearchParameters ρ σ)
-  (ctx : @SearchContext ρ σ κ σₕ List _ _ _ fp sys th hTh params)
+  (ctx : @SearchContext ρ σ κ σₕ fp sys th hTh params)
   : Trace ρ σ κ :=
   -- Get fingerprint traces from log
   let fingerprintTraces := collectTraces ctx
@@ -260,18 +258,18 @@ def recoverTrace {ρ σ κ σₕ : Type}
 
 def findReachable {ρ σ κ σₕ : Type}
   [fp : StateFingerprint σ σₕ]
-  [Inhabited κ] [Inhabited σ] [Repr σₕ]
+  [Inhabited κ] [Inhabited σ] [Repr σ] [Repr σₕ]
   [BEq ρ] [BEq σ] [BEq κ]
   (sys : EnumerableTransitionSystem ρ (List ρ) σ (List σ) κ (List (κ × σ)))
   (th : ρ) (hTh : th ∈ sys.theories)
   (params : SearchParameters ρ σ) : ReachabilityResult ρ σ κ :=
-  let ctx : @SearchContext ρ σ κ σₕ List _ _ _ fp sys th hTh params :=
-    breadthFirstSearch th hTh params
+  let ctx : @SearchContext ρ σ κ σₕ fp sys th hTh params :=
+    breadthFirstSearch sys th hTh params
   match ctx.finished with
-  | some StoppingCondition.foundViolatingState =>
+  | some (.earlyTermination .foundViolatingState) =>
     ReachabilityResult.reachable (some (recoverTrace sys th hTh params ctx))
-  | some StoppingCondition.exploredAllReachableStates =>
-    ReachabilityResult.unreachable
+  | some (.exploredAllReachableStates) =>
+    ReachabilityResult.unreachable ctx.seen.size
   | none =>
     ReachabilityResult.unknown
 
