Veil/Frontend/DSL/Module/Util.lean
@@ -800,7 +800,7 @@ def Module.declareStateFieldLabelTypeAndDispatchers [Monad m] [MonadQuotation m]
   -- NOTE: not actually needed, but left here for completeness to document what needs to exist
   -- let instances ← #[``Enumeration, ``Ord, ``ToJson].flatMapM fun inst => return (← mod.declareInstanceLiftingForDomain inst) ++ (← mod.declareInstanceLiftingForCodomain inst)
   let instances : Array Syntax := #[]
-  let concreteInstances ← #[(``Hashable, #[``DecidableEq, ``Ord, ``Hashable]), (``BEq, #[``DecidableEq, ``Ord]), (``ToJson, #[``ToJson, ``Ord])].flatMapM fun (deriveClass, assumingClasses) => mod.declareInstanceLiftingForConcreteType deriveClass assumingClasses
+  let concreteInstances ← #[(``Hashable, #[``DecidableEq, ``Ord, ``Hashable]), (``BEq, #[``DecidableEq, ``Ord]), (``ToJson, #[``ToJson, ``Ord]), (``Repr, #[``Repr, ``Ord])].flatMapM fun (deriveClass, assumingClasses) => mod.declareInstanceLiftingForConcreteType deriveClass assumingClasses
   -- add the `fieldConcreteType` parameter
   let fieldConcreteTypeParam ← Parameter.fieldConcreteType
   -- add the `FieldRepresentation` and `LawfulFieldRepresentation` typeclass parameters
